theories/typing/base_type.v
@@ -4,11 +4,8 @@ Set Default Proof Using "Type".
 Implicit Type 𝔄 𝔅: syn_type.
 
 (* [base] is a version of the empty type used internally in the model, using an
-   arbitrary refinement type. It is used for two purposes:
-     1- as a base case for the fixpoint (empty cannot be used since it is
-        using the empty semantic type).
-     2- as a default type in [sum.v] when performing lookups in lists of types
- *)
+  arbitrary refinement type. It is used for the base case of the fixpoint
+  type. *)
 
 Section base.
   Context `{!typeG Σ}.
