theories/typing/programs.v
@@ -361,8 +361,8 @@ Section typing.
   Qed.
 
   Lemma type_memcpy {𝔄 𝔄' 𝔅 𝔅' ℭ ℭ' 𝔄l 𝔅l 𝔇} (tyw: type 𝔄) (tyw': type 𝔄')
-    (tyr: type 𝔅) (tyr': type 𝔅') (tyb: type ℭ) (tyb': type ℭ') gtw stw gtr str Φ
-    (n: Z) pw pr E L (C: cctx 𝔇) (T: tctx 𝔄l) (T': tctx 𝔅l) e trx tr :
+      (tyr: type 𝔅) (tyr': type 𝔅') (tyb: type ℭ) (tyb': type ℭ') gtw stw gtr
+      str Φ (n: Z) pw pr E L (C: cctx 𝔇) (T: tctx 𝔄l) (T': tctx 𝔅l) e trx tr :
     Closed [] e → tctx_extract_ctx E L +[pw ◁ tyw; pr ◁ tyr] T T' trx →
     typed_write E L tyw tyb tyw' tyb' gtw stw → leak' E L tyb Φ →
     typed_read E L tyr tyb' tyr' gtr str → n = tyb'.(ty_size) →
