theories/typing/type_sum.v
@@ -1,440 +1,492 @@
 From iris.proofmode Require Import tactics.
 From lrust.lang Require Import memcpy.
-From lrust.typing Require Import uninit uniq_bor shr_bor own sum.
+From lrust.typing Require Import int uninit uniq_bor shr_bor own sum.
 From lrust.typing Require Import lft_contexts type_context programs product.
 From lrust.typing Require Import base_type.
 
 Set Default Proof Using "Type".
+Open Scope nat.
 
-Section case.
+Implicit Type (𝔄 𝔅: syn_type) (𝔄l 𝔅l: syn_typel).
+
+Notation sum_pad_size tyl ty := (max_ty_size tyl - ty.(ty_size))%nat.
+
+Section type_sum.
   Context `{!typeG Σ}.
 
-  Notation hnthb := (hnth (base (𝔄:=@empty _ Empty_setₛ_empty))).
+  (** * Owning Pointers *)
 
-  Lemma type_case_own' {ℭ 𝔄l 𝔅l} prel E L (C : cctx ℭ) (T : tctx 𝔅l)
-      p n (tyl : typel 𝔄l) el el' :
-    list_to_hlist el = Some el' →
-    HForallThree (λ _ ty e prei,
-      match prei with
-      | inl inner => ⊢ typed_body E L C
-          ((p +ₗ #0 ◁ own_ptr n (uninit 1)) +:: (p +ₗ #1 ◁ own_ptr n ty) +::
-            (p +ₗ #(S ty.(ty_size)) ◁ own_ptr n (uninit (max_ty_size tyl - ty_size ty))) +:: T)
-          e inner
-      | inr outer => ⊢ typed_body E L C ((p ◁ own_ptr n (xsum_ty tyl)) +:: T) e outer
-      end) tyl el' prel →
-    ⊢ typed_body E L C ((p ◁ own_ptr n (xsum_ty tyl)) +:: T) (case: !p of el)
-        (λ post '(v -:: w), ∀ i, match hnth (D := Empty_setₛ) (inr (λ _ _, False)) prel i with
-          | inl inner => ∀ v', v = pinj i v' → inner post (tt -:: v' -:: tt -:: w)
-          | inr outer => (∃ v', v = pinj (D := Empty_setₛ) i v') →  outer post (v -:: w)
-        end)%type.
+  Lemma tctx_unwrap_own_xsum {𝔄l 𝔅l} i (tyl: typel 𝔄l) n p (T: tctx 𝔅l) E L :
+    let tyi := tyl +!! i in
+    tctx_incl E L (p ◁ own_ptr n (Σ! tyl) +:: T)
+      (p +ₗ #0 ◁ own_ptr n int +:: p +ₗ #1 ◁ own_ptr n tyi +::
+        p +ₗ #(S tyi.(ty_size)) ◁ own_ptr n (↯ (sum_pad_size tyl tyi)) +:: T)
+      (λ post '(s -:: bl), ∃a: 𝔄l !!ₗ i,
+        s = pinj i a ∧ post (Z.of_nat i -:: a -:: () -:: bl)).
   Proof.
-    iIntros (elEl Hel tid [vπ vπl] postπ)
-      "#LFT #TIME #PROPH #UNIQ #HE Hna HL HC /= [Hp HT] Hproph".
-    wp_bind p. iApply (wp_hasty with "Hp").
-    iIntros ([[]|] [|depth1]) "%Hv #Hdepth Hp /= //".
-    iDestruct "Hp" as "[H↦ Hf]". iDestruct "H↦" as (vl) "[H↦ Hown]".
-    iMod (bi.later_exist_except_0 with "Hown") as (i) "Hown".
-    iMod (bi.later_exist_except_0 with "Hown")
-      as (wπ vl' vl'') "(>(% & % & EQlen) & Hown)". subst.
-    iDestruct "EQlen" as %[=EQlen]. rewrite -EQlen.
-    rewrite -(Nat.add_1_l (length _)) app_length -!freeable_sz_split /=
-            heap_mapsto_vec_cons heap_mapsto_vec_app.
-    iDestruct "H↦" as "(H↦i & H↦vl' & H↦vl'')". iDestruct "Hf" as "(Hfi & Hfvl' & Hfvl'')".
-    iAssert (⌜ i < length 𝔄l ⌝)%I with "[Hown]" as "%".
-    { case (decide (i < length 𝔄l)) => [//| ?].
-      rewrite hnth_default; [ apply lnth_default; lia | | lia].
-      move => eq. destruct eq; by pose proof (wπ inhabitant). }
-    eapply (HForallThree_nth_len _
-      (base (𝔄:=empty)) _ (inr (λ _ _, False)) _ _ _ i) in Hel as Hety; last lia.
-    wp_read. wp_case.
-    { split; [lia|]. destruct (list_to_hlist_length el el'); [done|].
-      edestruct (nth_lookup_or_length el i ltac:(done)); [|lia].
-      rewrite Nat2Z.id e. erewrite <-list_to_hlist_hnth_nth; [done|apply elEl]. }
-    destruct (hnth _ prel i) eqn:EQty.
-    - iApply (Hety $! tid (const () -:: _ -:: const () -:: _)
-                with "LFT TIME PROPH UNIQ HE Hna HL HC [-Hproph]").
-      rewrite /= !tctx_hasty_val' /= -?Hv //=; iFrame "HT".
-      + rewrite /own_ptr /=.
-        iDestruct (_.(ty_size_eq) with "Hown") as "%X". rewrite -X; clear X.
-        iSplitL "H↦i Hfi"; last iSplitR "H↦vl'' Hfvl''"; iExists _; iFrame "#"; simpl.
-        * rewrite shift_loc_0. iFrame. iExists [ #i]. rewrite heap_mapsto_vec_singleton.
-          auto with iFrame.
-        * eauto with iFrame.
-        * rewrite -EQlen app_length minus_plus shift_loc_assoc_nat. auto 10 with iFrame.
-      + iApply (proph_obs_impl with "Hproph") => π /= /(_ i).
-        rewrite EQty. auto.
-    - iApply (Hety $! tid (_ -:: _) with "LFT TIME PROPH UNIQ HE Hna HL HC [-Hproph]").
-      rewrite /= !tctx_hasty_val' /= -?Hv //=; iFrame "HT".
-      + iExists _. iFrame "#".
-        rewrite /= -EQlen app_length -(Nat.add_1_l (_+_)) -!freeable_sz_split. iFrame.
-        iExists (#i :: vl' ++ vl''). iNext.
-        rewrite heap_mapsto_vec_cons heap_mapsto_vec_app.
-        iFrame. iExists i,_, vl', vl''. rewrite /= app_length /=. auto.
-      + iApply (proph_obs_impl with "Hproph") => π /= /(_ i).
-        rewrite EQty. eauto.
+    split. { move=>/= ???[??]. by do 3 f_equiv. }
+    iIntros (??[??]?) "_ PROPH _ _ $ /=[p T] #Obs".
+    iDestruct "p" as ([[]|][|]Ev) "[#⧖ own]"=>//. rewrite/= split_sum_mt.
+    iDestruct "own" as "[big †]".
+    iMod (bi.later_exist_except_0 with "big") as (?) "big".
+    iMod (bi.later_exist_except_0 with "big") as (?) "(>->&(↦i &%& ↦p &><-)&%& ↦ & ty)".
+    rewrite -(Nat.add_1_l (_+_)) -!freeable_sz_split.
+    iDestruct "†" as "(†i & † & †p)". iDestruct (ty_size_eq with "ty") as "#>%Sz".
+    iMod (proph_obs_sat with "PROPH Obs") as %[?[?[Eq _]]]; [done|].
+    apply pinj_inj in Eq. move: Eq=> [? _]. subst. iModIntro.
+    iExists (const _-::_-::const ()-::_). iFrame "T". iSplit; last first.
+    { iApply proph_obs_impl; [|done]=>/= ?[?[Eq ?]]. apply pinj_Inj in Eq. by subst. }
+    iSplitL "↦i †i"; [|iSplitR "↦p †p"]; iExists _, _=>/=; rewrite Ev;
+    do 2 (iSplit; [done|]).
+    - rewrite shift_loc_0. iFrame "†i". iNext. iExists [_].
+      rewrite heap_mapsto_vec_singleton. iFrame "↦i". by iExists _.
+    - iFrame "†". iNext. iExists _. iFrame.
+    - iSplitL "↦p". { iNext. iExists _. iFrame "↦p". iPureIntro. lia. }
+      rewrite shift_loc_assoc_nat. iApply freeable_sz_eq; [|done]. lia.
   Qed.
 
-  Lemma type_case_own {ℭ 𝔄l 𝔅l ℭl} prel E L (C : cctx ℭ) (T : tctx 𝔅l) (T' : tctx ℭl)
-                      p n (tyl : typel 𝔄l) el el' fr :
-    list_to_hlist el = Some el' →
-    tctx_extract_ctx E L +[p ◁ own_ptr n (xsum_ty tyl)] T T' fr →
-    HForallThree (λ _ ty e prei,
-        match prei with
-        | inl inner => ⊢ typed_body E L C
-            ((p +ₗ #0 ◁ own_ptr n (uninit 1)) +:: (p +ₗ #1 ◁ own_ptr n ty) +::
-              (p +ₗ #(S ty.(ty_size)) ◁ own_ptr n (uninit (max_ty_size tyl - ty_size ty))) +:: T')
-            e inner
-        | inr outer => ⊢ typed_body E L C ((p ◁ own_ptr n (xsum_ty tyl)) +:: T') e outer
-        end) tyl el' prel →
-    ⊢ typed_body E L C T (case: !p of el)
-      (fr ∘ (λ post '(v -:: w), ∀ i, match hnth (D := Empty_setₛ) (inr (λ _ _, False)) prel i with
-        | inl inner => ∀ (v' : of_syn_type _), v = pinj i v' → inner post (tt -:: v' -:: tt -:: w)
-        | inr outer => (∃ (v' : of_syn_type _), v = pinj (D := Empty_setₛ) i v') → outer post (v -:: w)
-        end)%type).
-  Proof. intros. iApply typed_body_tctx_incl; [done|]. iApply type_case_own'; done. Qed.
-
-  Lemma type_case_uniq' {𝔄l ℭ 𝔅l} prel E L (C : cctx ℭ) (T : tctx 𝔅l) p κ (tyl : typel 𝔄l) el el' :
-    list_to_hlist el = Some el' → lctx_lft_alive E L κ →
-    HForallThree
-      (λ _ ty e prei, match prei with
-        | inl inner => ⊢ typed_body E L C ((p +ₗ #1 ◁ &uniq{κ}ty) +:: T) e inner
-        | inr outer => ⊢ typed_body E L C ((p ◁ &uniq{κ}(xsum_ty tyl)) +:: T) e outer
-        end) tyl el' prel →
-    ⊢ typed_body E L C ((p ◁ &uniq{κ}(xsum_ty tyl)) +:: T) (case: !p of el)
-        (λ post '(v -:: tl), ∀ i, match hnth (D := Empty_setₛ) (inr (λ _ _, False)) prel i with
-          | inl inner => ∀ (w w' : of_syn_type _), v = (pinj i w, pinj i w') → inner post ((w, w') -:: tl)
-          | inr outer => (∃ w, v.1 = pinj (D := Empty_setₛ) i w) →  outer post (v -:: tl)
-          end)%type.
+  Lemma type_case_own_outer {𝔄l 𝔅l ℭl 𝔇} (tyl: typel 𝔄l) trl (T: tctx 𝔅l)
+      (T': tctx ℭl) n p el el' trx E L (C: cctx 𝔇) :
+    IntoPlistc el el' →
+    tctx_extract_ctx E L +[p ◁ own_ptr n (Σ! tyl)] T T' trx →
+    ([∗ hlist] ty;- e; tr ∈ tyl;- el'; trl,
+      typed_body E L C (p ◁ own_ptr n (Σ! tyl) +:: T') e tr) -∗
+    typed_body E L C T (case: !p of el)
+      (trx ∘ (λ post '(s -:: cl), let 'xinj i _ := to_xsum s in
+        (trl -!! i) post (s -:: cl)))%type.
   Proof.
-    iIntros (el2el' Halive Hel tid [vπ vπl] postπ)
-      "#LFT #TIME #PROPH #UNIQ #HE Hna HL HC /= [Hp HT] Hproph".
-    wp_bind p. iApply (wp_hasty with "Hp").
-    iIntros ([[]|] [|depth1]) "%Hv #Hdepth /= [#? Hp] //".
-    { iDestruct "Hp" as (??) "(% & ?)". lia. }
-    iDestruct "Hp" as (depth2 ξid) "([% %B] & ξvo & Hp)"; set ξ := PrVar _ ξid.
-    iMod (Halive with "HE HL") as (q) "[Htok Hclose]"; [done|].
-    iMod (bor_acc_cons with "LFT Hp Htok") as "[H Hclose']"; [done|].
-    iMod (bi.later_exist_except_0 with "H") as (vπ' depth2') "(#Hdepth2' & ξpc & H↦)".
-    iDestruct "H↦" as (vl) "[> H↦ Hown]".
-    iMod (bi.later_exist_except_0 with "Hown") as (i) "Hown".
-    iMod (bi.later_exist_except_0 with "Hown") as (wπ vl' vl'') "(>(->&->& EQlen) & Hown)".
-    iMod (uniq_strip_later with "ξvo ξpc") as (A <-) "[ξvo ξpc]".
-    iDestruct "EQlen" as %[=EQlen].
-    rewrite heap_mapsto_vec_cons heap_mapsto_vec_app.
-    iDestruct "H↦" as "(H↦i & H↦vl' & H↦vl'')".
-    iAssert (⌜ i < length 𝔄l ⌝)%I with "[Hown]" as "%".
-    { clear -wπ. case (decide (i < length 𝔄l)) => [//| ?].
-      rewrite hnth_default; [ apply lnth_default; lia | | lia].
-      move => eq. destruct eq; by pose proof (wπ inhabitant). }
-    eapply (HForallThree_nth_len _ _ _ (inr (λ _ _, False)) _ _ _ i) in Hel as Hety; last lia.
-    wp_read. wp_case.
-    { split; [lia|]. destruct (list_to_hlist_length el el'); [done|].
-      edestruct (nth_lookup_or_length el i ltac:(done)); [|lia].
-      rewrite Nat2Z.id e. erewrite <-list_to_hlist_hnth_nth; [done|apply el2el']. }
-    iDestruct (_.(ty_size_eq) with "Hown") as %EQlenvl'.
-    destruct (hnth _ prel i) eqn:EQty.
-    - iMod (uniq_intro wπ depth2 with "PROPH UNIQ") as (ζid) "[ζvo ζpc]"; [done|].
-      set ζ := PrVar _ ζid.
-      iDestruct (uniq_proph_tok with "ζvo ζpc") as "(ζvo & ζ & Toζpc)".
-      rewrite proph_tok_singleton.
-      iMod (uniq_preresolve ξ _ (λ π, pinj i (π ζ)) with "PROPH ξvo ξpc ζ")
-        as "(#Hproph' & ζ & ξeqz)"; first done.
-      { apply proph_dep_constr, proph_dep_one. }
-      iDestruct ("Toζpc" with "ζ") as "ζpc".
-      iMod ("Hclose'" $! (∃ vπ' d', ⧖(S d') ∗ .PC[ζ] vπ' d' ∗
-          (l +ₗ 1) ↦∗: (hnthb tyl i).(ty_own) vπ' d' tid)%I
-        with "[ξeqz H↦i H↦vl''] [ ζpc H↦vl' Hown]") as "[Hb Htok]".
-      { iIntros "!>Hown".
-        iMod (bi.later_exist_except_0 with "Hown") as (??) "(#>Hdepth2'' & ζpc & Hown)".
-        iDestruct "Hown" as (vl'2) "[H↦ Hown]". iExists _, _. iModIntro; iNext.
-        iDestruct (proph_ctrl_eqz with "PROPH ζpc") as "ζeqz".
-        iDestruct (proph_eqz_constr (pinj i) with "ζeqz") as "ζeqz".
-        iDestruct ("ξeqz" with "ζeqz") as "ξpc".
-        iFrame "# ξpc". iExists (#i::vl'2++vl'').
-        iDestruct (_.(ty_size_eq) with "Hown") as %EQlenvl'2.
-        rewrite heap_mapsto_vec_cons heap_mapsto_vec_app EQlenvl' EQlenvl'2.
-        iFrame. iExists _, _, _, _. iFrame.
-        rewrite /= -EQlen !app_length EQlenvl' EQlenvl'2 //. }
-      { iNext. iExists _, _. iFrame "#∗". iExists _. iFrame. }
-      iMod ("Hclose" with "Htok") as "HL".
-      iApply (Hety $! _ ((λ π, (wπ π, π ζ)) -:: _) with
-        "LFT TIME PROPH UNIQ HE Hna HL HC [-Hproph]").
-      + iFrame. rewrite tctx_hasty_val' /= -?Hv //.
-        iExists (S depth1). iFrame "#". iSplitR.
-        { iApply lft_incl_trans; [done|]. iApply ty_lfts_nth_incl. }
-        rewrite (proof_irrel (_ wπ) (prval_to_inh' (λ π, (wπ π, π ζ)))).
-        iExists _, ζid. by iFrame.
-      + iCombine "Hproph' Hproph" as "Hproph".
-        iApply (proph_obs_impl with "Hproph") => π /= [+ /(_ i)].
-        move: (equal_f A π) (equal_f B π).
-        rewrite EQty {5}(_ : vπ = λ π, (fst (vπ π), snd (vπ π))); last first.
-        { fun_ext => π'. by destruct (vπ π'). }
-        move => /=->->->. auto.
-    - iMod ("Hclose'" with "[] [H↦i H↦vl' H↦vl'' Hown ξpc]") as "[Hb Htok]";
-        [by iIntros "!>$"| |].
-      { iExists _, depth2. iFrame "∗#". iExists (#i::vl'++vl'').
-        rewrite heap_mapsto_vec_cons heap_mapsto_vec_app /= -EQlen.
-        iFrame. iNext. iExists i, _, vl', vl''. by iFrame. }
-      iMod ("Hclose" with "Htok") as "HL".
-      iApply (Hety $! _ (_ -:: _) with "LFT TIME PROPH UNIQ HE Hna HL HC [-Hproph]").
-      + iFrame. rewrite tctx_hasty_val' ?Hv //. iExists (S depth1).
-        iFrame "#". iExists _, _. auto with iFrame.
-      + iApply (proph_obs_impl with "Hproph") => π /= /(_ i).
-        move: (equal_f A π). rewrite EQty => /= ->. eauto.
+    move=> ->. iIntros (?) "el". iApply typed_body_tctx_incl; [done|].
+    iIntros (?[??]?) "LFT TIME PROPH UNIQ E Na L C /=[p T] #?".
+    wp_apply (wp_hasty with "p"). iIntros ([[]|][|]?) "#⧖ own"=>//.
+    iDestruct "own" as "[(%& >↦ & big) †]".
+    iMod (bi.later_exist_except_0 with "big") as (?) "big".
+    iMod (bi.later_exist_except_0 with "big") as (aπ ??) "[>(->&->&%) ty]".
+    rewrite heap_mapsto_vec_cons. iDestruct "↦" as "[↦i ↦]". wp_read. wp_case.
+    { split; [lia|]. by rewrite Nat2Z.id -vlookup_lookup plistc_to_vec_lookup. }
+    rewrite big_sepHL_2_lookup. iApply ("el" $! _ ((λ π, _) -:: _) with
+      "LFT TIME PROPH UNIQ E Na L C [-] []"); last first.
+    { iApply proph_obs_impl; [|done]=>/= ?. by rewrite to_xsum_pinj. }
+    iFrame "T". iExists _, _. iSplit; [done|]. iFrame "⧖ †". iNext.
+    iExists (_::_). rewrite heap_mapsto_vec_cons. iFrame "↦ ↦i".
+    iExists _, _, _, _. by iFrame "ty".
   Qed.
 
-  Lemma type_case_uniq {ℭ 𝔄l 𝔅l ℭl} prel E L (C : cctx ℭ) (T : tctx 𝔅l) (T' : tctx ℭl)
-                       p κ (tyl : typel 𝔄l) el el' fr :
-    list_to_hlist el = Some el' → lctx_lft_alive E L κ →
-    tctx_extract_ctx E L +[p ◁ &uniq{κ}(xsum_ty tyl)] T T' fr →
+  Lemma type_case_own {𝔄l 𝔅l ℭl 𝔇} (tyl: typel 𝔄l) trl (T: tctx 𝔅l)
+      (T': tctx ℭl) n p el el' trx E L (C: cctx 𝔇) :
+    IntoPlistc el el' →
+    tctx_extract_ctx E L +[p ◁ own_ptr n (Σ! tyl)] T T' trx →
+    ([∗ hlist] ty;- e; tr ∈ tyl;- el'; trl, match tr with
+      | inl otr => typed_body E L C (p ◁ own_ptr n (Σ! tyl) +:: T') e otr
+      | inr itr => typed_body E L C
+          (p +ₗ #0 ◁ own_ptr n int +:: p +ₗ #1 ◁ own_ptr n ty +::
+            p +ₗ #(S ty.(ty_size)) ◁ own_ptr n (↯ (sum_pad_size tyl ty)) +:: T') e itr
+      end) -∗
+    typed_body E L C T (case: !p of el) (trx ∘ (λ post '(s -:: cl),
+      let 'xinj i a := to_xsum s in match trl -!! i with
+        | inl otr => otr post (s -:: cl)
+        | inr itr => itr post (Z.of_nat i -:: a -:: () -:: cl)
+        end)).
+  Proof.
+    iIntros (??) "el". iApply typed_body_tctx_incl; [done|]. via_tr_impl.
+    { iApply (type_case_own_outer _ (pbyidx (λ i post '(s -:: cl),
+        match trl -!! i with inl otr => otr post (s -:: cl) | inr itr => _ end
+        : Prop))); [apply tctx_incl_refl|].
+      rewrite !big_sepHL_2_big_sepN. iApply (big_sepN_impl with "el").
+      iIntros "!>" (i) "?". rewrite pbyidx_plookup.
+      case (trl -!! i)=> ?; [by via_tr_impl; [done|]=> ?[??]?|]. via_tr_impl.
+      { iApply typed_body_tctx_incl; [apply tctx_unwrap_own_xsum|done]. }
+      move=>/= ?[??]. exact id. }
+    move=> ?[s ?]/=. case (to_xsum s) as [i ?] eqn: Eq. rewrite pbyidx_plookup.
+    move: (trl -!! i). case; [done|]=>/= ??. eexists _. split; [|done].
+    move: Eq=> /(f_equal of_xsum)=>/= <-. by rewrite semi_iso'.
+  Qed.
+
+  Lemma type_case_own_inner {𝔄l 𝔅l ℭl 𝔇} (tyl: typel 𝔄l) trl (T: tctx 𝔅l)
+      (T': tctx ℭl) n p el el' trx E L (C: cctx 𝔇) :
+    IntoPlistc el el' →
+    tctx_extract_ctx E L +[p ◁ own_ptr n (Σ! tyl)] T T' trx →
+    ([∗ hlist] ty;- e; tr ∈ tyl;- el'; trl,
+      typed_body E L C (p +ₗ #0 ◁ own_ptr n int +:: p +ₗ #1 ◁ own_ptr n ty +::
+        p +ₗ #(S ty.(ty_size)) ◁ own_ptr n (↯ (sum_pad_size tyl ty)) +:: T') e tr) -∗
+    typed_body E L C T (case: !p of el) (trx ∘ (λ post '(s -:: cl),
+      let 'xinj i a := to_xsum s in
+      (trl -!! i) post (Z.of_nat i -:: a -:: () -:: cl))).
+  Proof.
+    iIntros (??) "el". iApply typed_body_tctx_incl; [done|]. via_tr_impl.
+    { iApply (type_case_own _ (pbyidx (λ i, inr (trl -!! i)))); [solve_typing|].
+      rewrite !big_sepHL_2_big_sepN. iApply (big_sepN_impl with "el").
+      iIntros "!>" (?) "?". by rewrite pbyidx_plookup. }
+    move=> ?[s ?]/=. case (to_xsum s)=>/= ??. by rewrite pbyidx_plookup.
+  Qed.
+
+  (** * Shared References *)
+
+  Lemma tctx_unwrap_shr_xsum {𝔄l 𝔅l} i (tyl: typel 𝔄l) κ p (T: tctx 𝔅l) E L :
+    tctx_incl E L (p ◁ &shr{κ} (Σ! tyl) +:: T) (p +ₗ #1 ◁ &shr{κ} (tyl +!! i) +:: T)
+      (λ post '(s -:: bl), ∃a: 𝔄l !!ₗ i, s = pinj i a ∧ post (a -:: bl)).
+  Proof.
+    split. { move=>/= ???[??]. by do 3 f_equiv. }
+    iIntros (??[??]?) "_ PROPH _ _ $ /=[p T] #Obs".
+    iMod (proph_obs_sat with "PROPH Obs") as %[?[?[Eq _]]]; [done|]. iModIntro.
+    iDestruct "p" as ([[]|][|]Ev) "[#⧖ sum]"=>//.
+    iDestruct "sum" as (??->) "[_ ty]". apply pinj_inj in Eq. move: Eq=> [??].
+    subst. iExists (_-::_). iFrame "T". iSplit.
+    { iExists _, _. iSplit; [by rewrite/= Ev|]. iFrame "⧖ ty". }
+    iApply proph_obs_impl; [|done]=>/= ?[?[Eq ?]]. apply pinj_Inj in Eq. by subst.
+  Qed.
+
+  Lemma type_case_shr_outer {𝔄l 𝔅l ℭl 𝔇} (tyl: typel 𝔄l) trl (T: tctx 𝔅l)
+      (T': tctx ℭl) κ p el el' trx E L (C: cctx 𝔇) :
+    IntoPlistc el el' →
+    tctx_extract_ctx E L +[p ◁ &shr{κ} (Σ! tyl)] T T' trx → lctx_lft_alive E L κ →
+    ([∗ hlist] ty;- e; tr ∈ tyl;- el'; trl,
+      typed_body E L C (p ◁ &shr{κ} (Σ! tyl) +:: T') e tr) -∗
+    typed_body E L C T (case: !p of el)
+      (trx ∘ (λ post '(s -:: cl), let 'xinj i _ := to_xsum s in
+        (trl -!! i) post (s -:: cl)))%type.
+  Proof.
+    move=> ->. iIntros (? Alv) "el". iApply typed_body_tctx_incl; [done|].
+    iIntros (?[??]?) "#LFT TIME PROPH UNIQ #E Na L C /=[p T] #?".
+    wp_apply (wp_hasty with "p"). iIntros ([[]|][|]?) "#⧖ sum"=>//.
+    iDestruct "sum" as (??->) "[#Bor ty]".
+    iMod (Alv with "E L") as (?) "[κ ToL]"; [done|].
+    iMod (frac_bor_acc with "LFT Bor κ") as (?) "[[>↦i ↦p] Toκ]"; [done|].
+    wp_read. iMod ("Toκ" with "[$↦i $↦p]") as "κ". iMod ("ToL" with "κ") as "L".
+    wp_case. { split; [lia|]. by rewrite Nat2Z.id -vlookup_lookup plistc_to_vec_lookup. }
+    rewrite big_sepHL_2_lookup. iApply ("el" $! _ ((λ π, _) -:: _) with
+      "LFT TIME PROPH UNIQ E Na L C [-] []"); last first.
+    { iApply proph_obs_impl; [|done]=>/= ?. by rewrite to_xsum_pinj. }
+    iFrame "T". iExists _, _. iSplit; [done|]. iFrame "⧖". iExists _, _.
+    by iFrame "Bor ty".
+  Qed.
+
+  Lemma type_case_shr {𝔄l 𝔅l ℭl 𝔇} (tyl: typel 𝔄l) trl (T: tctx 𝔅l)
+      (T': tctx ℭl) κ p el el' trx E L (C: cctx 𝔇) :
+    IntoPlistc el el' →
+    tctx_extract_ctx E L +[p ◁ &shr{κ} (Σ! tyl)] T T' trx → lctx_lft_alive E L κ →
+    ([∗ hlist] ty;- e; tr ∈ tyl;- el'; trl, match tr with
+      | inl otr => typed_body E L C (p ◁ &shr{κ} (Σ! tyl) +:: T') e otr
+      | inr itr => typed_body E L C (p +ₗ #1 ◁ &shr{κ} ty +:: T') e itr
+      end) -∗
+    typed_body E L C T (case: !p of el) (trx ∘ (λ post '(s -:: cl),
+      let 'xinj i a := to_xsum s in match trl -!! i with
+        | inl otr => otr post (s -:: cl)
+        | inr itr => itr post (a -:: cl)
+        end)).
+  Proof.
+    iIntros (???) "el". iApply typed_body_tctx_incl; [done|]. via_tr_impl.
+    { iApply (type_case_shr_outer _ (pbyidx (λ i post '(s -:: cl),
+        match trl -!! i with inl otr => otr post (s -:: cl) | inr itr => _ end
+        : Prop))); [apply tctx_incl_refl|done|].
+      rewrite !big_sepHL_2_big_sepN. iApply (big_sepN_impl with "el").
+      iIntros "!>" (i) "?". rewrite pbyidx_plookup.
+      case (trl -!! i)=> ?; [by via_tr_impl; [done|]=> ?[??]?|]. via_tr_impl.
+      { iApply typed_body_tctx_incl; [apply tctx_unwrap_shr_xsum|done]. }
+      move=>/= ?[??]. exact id. }
+    move=> ?[s ?]/=. case (to_xsum s) as [i ?] eqn: Eq. rewrite pbyidx_plookup.
+    move: (trl -!! i). case; [done|]=>/= ??. eexists _. split; [|done].
+    move: Eq=> /(f_equal of_xsum)=>/= <-. by rewrite semi_iso'.
+  Qed.
+
+  Lemma type_case_shr_inner {𝔄l 𝔅l ℭl 𝔇} (tyl: typel 𝔄l) trl (T: tctx 𝔅l)
+      (T': tctx ℭl) κ p el el' trx E L (C: cctx 𝔇) :
+    IntoPlistc el el' →
+    tctx_extract_ctx E L +[p ◁ &shr{κ} (Σ! tyl)] T T' trx → lctx_lft_alive E L κ →
+    ([∗ hlist] ty;- e; tr ∈ tyl;- el'; trl,
+      typed_body E L C (p +ₗ #1 ◁ &shr{κ} ty +:: T') e tr) -∗
+    typed_body E L C T (case: !p of el) (trx ∘ (λ post '(s -:: cl),
+      let 'xinj i a := to_xsum s in (trl -!! i) post (a -:: cl))).
+  Proof.
+    iIntros (???) "el". iApply typed_body_tctx_incl; [done|]. via_tr_impl.
+    { iApply (type_case_shr _ (pbyidx (λ i, inr (trl -!! i))));
+        [apply tctx_incl_refl|done|].
+      rewrite !big_sepHL_2_big_sepN. iApply (big_sepN_impl with "el").
+      iIntros "!>" (?) "?". by rewrite pbyidx_plookup. }
+    move=> ?[s ?]/=. case (to_xsum s)=>/= ??. by rewrite pbyidx_plookup.
+  Qed.
+
+  (** * Unique References *)
+
+  Lemma tctx_unwrap_uniq_xsum {𝔄l 𝔅l} i (tyl: typel 𝔄l) κ p (T: tctx 𝔅l) E L :
     lctx_lft_alive E L κ →
-    HForallThree
-      (λ _ ty e prei, match prei with
-        | inl x => ⊢ typed_body E L C ((p +ₗ #1 ◁ &uniq{κ}ty) +:: T') e x
-        | inr y => ⊢ typed_body E L C ((p ◁ &uniq{κ}(xsum_ty tyl)) +:: T') e y
-        end) tyl el' prel →
-    ⊢ typed_body E L C T (case: !p of el)
-        (fr ∘ (λ post '(v -:: tl), ∀ i, match hnth (D := Empty_setₛ) (inr (λ _ _, False)) prel i with
-        | inl inner => ∀ (w w' : of_syn_type _), v = (pinj i w, pinj i w') → inner post ((w, w') -:: tl)
-        | inr outer => (∃ w, v.1 = pinj (D := Empty_setₛ) i w) →  outer post (v -:: tl)
-        end)%type).
-  Proof. intros. iApply typed_body_tctx_incl; [done|]. iApply type_case_uniq'; done. Qed.
-
-  Lemma type_case_shr' {𝔅l 𝔄l ℭ} prel E L (C : cctx ℭ) (T : tctx 𝔅l) p κ (tyl : typel 𝔄l) el el' :
-    list_to_hlist el = Some el' → lctx_lft_alive E L κ →
-    HForallThree (λ _ ty e prei,
-      match prei with
-      | inl inner => ⊢ typed_body E L C ((p +ₗ #1 ◁ &shr{κ}ty) +:: T) e inner
-      | inr outer => ⊢ typed_body E L C ((p ◁ &shr{κ}(xsum_ty tyl)) +:: T) e outer
-      end) tyl el' prel →
-    ⊢ typed_body E L C ((p ◁ &shr{κ}(xsum_ty tyl)) +:: T) (case: !p of el)
-      (λ post '(v -:: w), ∀ i, match hnth (D := Empty_setₛ) (inr (λ _ _, False)) prel i with
-        | inl inner => ∀ v', v = pinj i v' → inner post (v' -:: w)
-        | inr outer => (∃ w, v = pinj (D := Empty_setₛ) i w) →  outer post (v -:: w)
-      end)%type.
+    tctx_incl E L (p ◁ &uniq{κ} (Σ! tyl) +:: T) (p +ₗ #1 ◁ &uniq{κ} (tyl +!! i) +:: T)
+      (λ post '((s, s') -:: bl), ∃a: 𝔄l !!ₗ i, s = pinj i a ∧
+        ∀a': 𝔄l !!ₗ i, s' = pinj i a' → post ((a, a') -:: bl)).
   Proof.
-    iIntros (el2el' Halive Hel tid [? ?] postπ)
-      "#LFT #TIME #PROPH UNIQ #HE Hna HL HC /= [Hp HT] Hproph".
-    wp_bind p. iApply (wp_hasty with "Hp").
-    iIntros ([[]|] [|depth]) "% Hdepth Hp //".
-    iDestruct "Hp" as (i vπ) "(%Hvπ & #Hb & Hshr)".
-    iMod (Halive with "HE HL") as (q) "[Htok Hclose]". done.
-    iMod (frac_bor_acc with "LFT Hb Htok") as (q') "[[H↦i H↦vl''] Hclose']". done.
-    iAssert (⌜ i < length 𝔄l ⌝)%I with "[Hshr]" as "%".
-    { clear -vπ. case (decide (i < length 𝔄l)) => [//| ?].
-      rewrite hnth_default; [ apply lnth_default; lia | | lia].
-      move => eq; destruct eq; by pose proof (vπ inhabitant). }
-    eapply (HForallThree_nth_len _ _ _ (inr (λ _ _, False)) _ _ _ i) in Hel as Hety; last lia.
-    wp_read. wp_case.
-    { split; [lia|]. destruct (list_to_hlist_length el el'); [done|].
-      edestruct (nth_lookup_or_length el i ltac:(done)); [|lia].
-      rewrite Nat2Z.id e. erewrite <-list_to_hlist_hnth_nth; [done|apply el2el']. }
-    iMod ("Hclose'" with "[$H↦i $H↦vl'']") as "Htok".
-    iMod ("Hclose" with "Htok") as "HL".
-    destruct (hnth _ prel i) eqn:EQty;
-    iApply (Hety $! _ (_ -:: _) with "LFT TIME PROPH UNIQ HE Hna HL HC [-Hproph]").
-    - rewrite /= tctx_hasty_val' /= -?H //. iFrame. iExists _. by iFrame.
-    - iApply (proph_obs_impl with "Hproph") => /= π /(_ i); rewrite Hvπ EQty; eauto.
-    - rewrite /= tctx_hasty_val' /= -?H //. iFrame.
-      iExists _. iFrame. iExists _, _. by iFrame "%∗".
-    - iApply (proph_obs_impl with "Hproph") => /= π /(_ i); rewrite Hvπ EQty; eauto.
+    move=> Alv. split.
+    { move=>/= ???[[??]?]. do 3 f_equiv. by do 2 (apply forall_proper=> ?). }
+    iIntros (??[vπ ?]?) "LFT #PROPH UNIQ E L /=[p T] #Obs".
+    iDestruct "p" as ([[]|]? Ev) "(_&#?& uniq)"=>//.
+    iDestruct "uniq" as (? ξi [? Eq2]) "[Vo Bor]". set ξ := PrVar _ ξi.
+    iMod (Alv with "E L") as (?) "[κ ToL]"; [done|].
+    iMod (bor_acc_cons with "LFT Bor κ") as "[big ToBor]" ; [done|].
+    iMod (bi.later_exist_except_0 with "big") as (??) "(>#⧖ & Pc & big)".
+    rewrite split_sum_mt. iMod (bi.later_exist_except_0 with "big") as (i') "big".
+    iMod (bi.later_exist_except_0 with "big") as (aπ) "(>->& ↦ip &%& >↦ & ty)".
+    iMod (uniq_strip_later with "Vo Pc") as (Eq1 <-) "[Vo Pc]".
+    have ->: vπ = λ π, (pinj i' (aπ π), π ξ).
+    { by rewrite [vπ]surjective_pairing_fun Eq1 Eq2. }
+    iMod (proph_obs_sat with "PROPH Obs") as %[?[?[Eq _]]]; [done|].
+    apply pinj_inj in Eq. move: Eq=> [? _]. subst.
+    iMod (uniq_intro aπ with "PROPH UNIQ") as (ζi) "[Vo' Pc']"; [done|].
+    set ζ := PrVar _ ζi. iDestruct (uniq_proph_tok with "Vo' Pc'") as "(Vo' & ζ & Pc')".
+    iMod (uniq_preresolve ξ [ζ] (λ π, pinj i (π ζ)) with "PROPH Vo Pc [$ζ]")
+      as "(Obs' &[ζ _]& ToPc)"; [done|by apply proph_dep_constr, proph_dep_one|done|].
+    iCombine "Obs' Obs" as "#?". iClear "Obs". iSpecialize ("Pc'" with "ζ").
+    iMod ("ToBor" with "[↦ip ToPc] [↦ ty Pc']") as "[Bor κ]"; last first.
+    - iMod ("ToL" with "κ") as "$". iModIntro.
+      iExists ((λ π, (aπ π, π ζ)) -::_). iFrame "T". iSplitL.
+      { iExists _, _. iSplit; [by rewrite/= Ev|]. iFrame "⧖". iSplit.
+        { iApply lft_incl_trans; [done|]. iApply ty_lfts_lookup_incl. }
+        iExists _, _. by iFrame. }
+      iApply proph_obs_impl; [|done]=>/= ?[?[?[Eq All]]]. apply pinj_Inj in Eq.
+      subst. by apply All.
+    - iNext. iExists _, _. iFrame "⧖ Pc'". iExists _. iFrame.
+    - iIntros "!> big !>!>". iDestruct "big" as (??) "(⧖' & Pc' &%& ↦ & ty)".
+      iExists _, _. iFrame "⧖'". iSplitL "Pc' ToPc".
+      { iApply "ToPc". iApply proph_eqz_constr. by iApply proph_ctrl_eqz. }
+      rewrite split_sum_mt. iExists _, _. iSplit; [done|]. iFrame "↦ip".
+      iExists _. iFrame.
   Qed.
 
-  Lemma type_case_shr {ℭ 𝔄l 𝔅l ℭl} prel E L (C : cctx ℭ) (T : tctx 𝔅l) (T' : tctx ℭl)
-                      p κ (tyl : typel 𝔄l) el el' fr :
-    list_to_hlist el = Some el' → lctx_lft_alive E L κ →
-    tctx_extract_ctx E L +[p ◁ &shr{κ}(xsum_ty tyl)] T T' fr →
-    HForallThree (λ _ ty e prei,
-      match prei with
-      | inl inner => ⊢ typed_body E L C ((p +ₗ #1 ◁ &shr{κ}ty) +:: T') e inner
-      | inr outer => ⊢ typed_body E L C ((p ◁ &shr{κ}(xsum_ty tyl)) +:: T') e outer
-      end) tyl el' prel →
-    ⊢ typed_body E L C T (case: !p of el)
-        (fr ∘ (λ post '(v -:: w), ∀ i, match hnth (D := Empty_setₛ) (inr (λ _ _, False)) prel i with
-            | inl inner => ∀ v', v = pinj i v' → inner post (v' -:: w)
-            | inr outer => (∃ w, v = pinj (D := Empty_setₛ) i w) → outer post (v -:: w)
-          end)%type).
-  Proof. intros. iApply typed_body_tctx_incl; [done|]. iApply type_case_shr'; done. Qed.
+  Lemma type_case_uniq_outer {𝔄l 𝔅l ℭl 𝔇} (tyl: typel 𝔄l) trl (T: tctx 𝔅l)
+      (T': tctx ℭl) κ p el el' trx E L (C: cctx 𝔇) :
+    IntoPlistc el el' →
+    tctx_extract_ctx E L +[p ◁ &uniq{κ} (Σ! tyl)] T T' trx → lctx_lft_alive E L κ →
+    ([∗ hlist] ty;- e; tr ∈ tyl;- el'; trl,
+      typed_body E L C (p ◁ &uniq{κ} (Σ! tyl) +:: T') e tr) -∗
+    typed_body E L C T (case: !p of el)
+      (trx ∘ (λ post '((s, s') -:: cl), let 'xinj i _ := to_xsum s in
+        (trl -!! i) post ((s, s') -:: cl)))%type.
+  Proof.
+    move=> ->. iIntros (? Alv) "el". iApply typed_body_tctx_incl; [done|].
+    iIntros (?[vπ ?]?) "#LFT TIME PROPH UNIQ #E Na L C /=[p T] #?".
+    wp_apply (wp_hasty with "p"). iIntros ([[]|]??) "_ [#In uniq]"=>//.
+    iDestruct "uniq" as (? ξi [??]) "[Vo Bor]". set ξ := PrVar _ ξi.
+    iMod (Alv with "E L") as (?) "[κ ToL]"; [done|].
+    iMod (bor_acc with "LFT Bor κ") as "[big ToBor]"; [done|].
+    iMod (bi.later_exist_except_0 with "big") as (??) "(#⧖ & Pc & big)".
+    rewrite split_sum_mt. iMod (bi.later_exist_except_0 with "big") as (i) "big".
+    iMod (bi.later_exist_except_0 with "big") as (aπ) "(>->& [>↦i ↦p] & ↦ty)".
+    wp_read. iDestruct (uniq_agree with "Vo Pc") as %[Eq <-].
+    iMod ("ToBor" with "[Pc ↦i ↦p ↦ty]") as "[Bor κ]".
+    { iNext. iExists _, _. iFrame "⧖ Pc". rewrite split_sum_mt. iExists _, _. by iFrame. }
+    iMod ("ToL" with "κ") as "L". wp_case.
+    { split; [lia|]. by rewrite Nat2Z.id -vlookup_lookup plistc_to_vec_lookup. }
+    rewrite big_sepHL_2_lookup. iApply ("el" $! _ (vπ -:: _) with
+      "LFT TIME PROPH UNIQ E Na L C [-] []"); last first.
+    { iApply proph_obs_impl; [|done]=>/= π. move: (equal_f Eq π)=>/=.
+      case (vπ π)=>/= ??->. by rewrite to_xsum_pinj. }
+    iFrame "T". iExists _, _. iSplit; [done|]. iFrame "⧖ In". iExists _, _. by iFrame.
+  Qed.
 
-  Lemma type_sum_assign_instr {E L 𝔄 𝔄' 𝔅 𝔄l} (i : nat) (ty1: type 𝔄)
-                              (ty' : type 𝔅) (tyl: typel 𝔄l) (ty2: type 𝔄') p1 p2 gt st Φ:
-    typed_write E L ty1 ty' ty2 (xsum_ty tyl) gt st  →
-    leak' E L ty' Φ →
-    typed_instr E L +[p1 ◁ ty1; p2 ◁ hnthb tyl i] (p1 <-{Σ i} p2) (λ _, +[p1 ◁ ty2])
+  Lemma type_case_uniq {𝔄l 𝔅l ℭl 𝔇} (tyl: typel 𝔄l) trl (T: tctx 𝔅l)
+      (T': tctx ℭl) κ p el el' trx E L (C: cctx 𝔇) :
+    IntoPlistc el el' →
+    tctx_extract_ctx E L +[p ◁ &uniq{κ} (Σ! tyl)] T T' trx → lctx_lft_alive E L κ →
+    ([∗ hlist] ty;- e; tr ∈ tyl;- el'; trl, match tr with
+      | inl otr => typed_body E L C (p ◁ &uniq{κ} (Σ! tyl) +:: T') e otr
+      | inr itr => typed_body E L C (p +ₗ #1 ◁ &uniq{κ} ty +:: T') e itr
+      end) -∗
+    typed_body E L C T (case: !p of el) (trx ∘ (λ post '((s, s') -:: cl),
+      let 'xinj i a := to_xsum s in match trl -!! i with
+        | inl otr => otr post ((s, s') -:: cl)
+        | inr itr => ∀a': 𝔄l !!ₗ i, s' = pinj i a' → itr post ((a, a') -:: cl)
+        end))%type.
+  Proof.
+    iIntros (???) "el". iApply typed_body_tctx_incl; [done|]. via_tr_impl.
+    { iApply (type_case_uniq_outer _ (pbyidx (λ i post '((s, s') -:: cl),
+        match trl -!! i with inl otr => otr post ((s, s') -:: cl) | inr itr => _ end
+        : Prop))); [apply tctx_incl_refl|done|].
+      rewrite !big_sepHL_2_big_sepN. iApply (big_sepN_impl with "el").
+      iIntros "!>" (i) "?". rewrite pbyidx_plookup.
+      case (trl -!! i)=> ?; [by via_tr_impl; [done|]=> ?[[??]?]?|]. via_tr_impl.
+      { iApply typed_body_tctx_incl; [by apply tctx_unwrap_uniq_xsum|done]. }
+      move=>/= ?[[??]?]. exact id. }
+    move=> ?[[s ?]?]/=. case (to_xsum s) as [i ?] eqn: Eq. rewrite pbyidx_plookup.
+    move: (trl -!! i). case; [done|]=>/= ??. eexists _. split; [|done].
+    move: Eq=> /(f_equal of_xsum)=>/= <-. by rewrite semi_iso'.
+  Qed.
+
+  Lemma type_case_uniq_inner {𝔄l 𝔅l ℭl 𝔇} (tyl: typel 𝔄l) trl (T: tctx 𝔅l)
+      (T': tctx ℭl) κ p el el' trx E L (C: cctx 𝔇) :
+    IntoPlistc el el' →
+    tctx_extract_ctx E L +[p ◁ &uniq{κ} (Σ! tyl)] T T' trx → lctx_lft_alive E L κ →
+    ([∗ hlist] ty;- e; tr ∈ tyl;- el'; trl,
+      typed_body E L C (p +ₗ #1 ◁ &uniq{κ} ty +:: T') e tr) -∗
+    typed_body E L C T (case: !p of el) (trx ∘ (λ post '((s, s') -:: cl),
+      let 'xinj i a := to_xsum s in
+      ∀a': 𝔄l !!ₗ i, s' = pinj i a' → (trl -!! i) post ((a, a') -:: cl)))%type.
+  Proof.
+    iIntros (???) "el". iApply typed_body_tctx_incl; [done|]. via_tr_impl.
+    { iApply (type_case_uniq _ (pbyidx (λ i, inr (trl -!! i))));
+        [apply tctx_incl_refl|done|].
+      rewrite !big_sepHL_2_big_sepN. iApply (big_sepN_impl with "el").
+      iIntros "!>" (?) "?". by rewrite pbyidx_plookup. }
+    move=> ?[[s ?]?]/=. case (to_xsum s)=>/= ??. by rewrite pbyidx_plookup.
+  Qed.
+
+  (** * Write *)
+
+  Lemma type_sum_assign_instr {𝔄 𝔄' 𝔅 𝔅l} (tyl: typel 𝔅l) (i: fin _)
+      (ty: type 𝔄) (tyb: type 𝔅) (ty': type 𝔄')  p q gt st Φ E L :
+    typed_write E L ty tyb ty' (Σ! tyl) gt st → leak' E L tyb Φ →
+    typed_instr E L +[p ◁ ty; q ◁ tyl +!! i] (p <-{Σ i} q) (λ _, +[p ◁ ty'])
       (λ post '-[a; b], Φ (gt a) (post -[st a (pinj i b)])).
   Proof.
-    iIntros ([Eq Hw] Lk tid postπ (? & ? & []))
-      "#LFT #TIME #PROPH #UNIQ #HE $ [HL HL'] (Hp1 & Hp2 & _) Hproph".
-    iDestruct (closed_hasty with "Hp1") as "%". iDestruct (closed_hasty with "Hp2") as "%".
-    wp_apply (wp_hasty with "Hp1"). iIntros (v1 depth1) "%Hv1 Hdepth1 Hty1".
-    iDestruct "Hp2" as (v2 depth2) "(%Hv2 & Hdepth2 & Hty2)".
-    iCombine "Hdepth1 Hdepth2" as "#Hdepth".
-    rewrite !(ty_own_depth_mono _ _ (depth1 `max` depth2)); [|lia..].
-    iMod (Hw with "LFT UNIQ HE HL Hty1") as (l ->) "(H & Hw)".
-    iDestruct "H" as (vl) "(> H↦ & Leaked)".
-    iAssert (▷ (ty_own ty' (gt ∘ phd) (depth1 `max` depth2) tid vl ∗
-      ⌜length vl = ty_size ty'⌝) )%I with "[Leaked]" as "[Leaked >%Hlen]".
-    { iNext. iDestruct (ty_size_eq with "Leaked") as %<-. by iFrame. }
-    destruct vl as [|? vl]; rewrite Eq //= in Hlen. rewrite heap_mapsto_vec_cons.
-    iDestruct (Lk (⊤ ∖ (⊤ ∖ ↑lftN ∖ ↑prophN)) with "LFT PROPH HE HL' Leaked") as "ToObs";
-      first set_solver.
-    iApply (wp_step_fupdN_persistent_time_receipt _ _ (⊤ ∖ ↑lftN ∖ ↑prophN)
-    with "TIME Hdepth [ToObs]")=>//. { by iApply step_fupdN_with_emp. }
-    iDestruct "H↦" as "[H↦0 H↦vl]".
-    wp_write. wp_bind p1. iApply (wp_wand with "[]"); first by iApply (wp_eval_path).
-    iIntros (? ->). wp_op. wp_bind p2.
-    iApply (wp_wand with "[]"); first by iApply (wp_eval_path). iIntros (? ->).
-    iDestruct (ty_size_eq with "Hty2") as %Hlenty. destruct vl as [|? vl].
-    { exfalso. move: (Hlen) (i) Hlenty. elim tyl => //= > IH ? [|?]; eauto with lia.  }
-    rewrite heap_mapsto_vec_cons -wp_fupd.
-    iApply (wp_persistent_time_receipt with "TIME Hdepth"); first solve_ndisj.
-    iDestruct "H↦vl" as "[H↦ H↦vl]". wp_write. iIntros "#Hdepth' !> [ToObs HL']".
-    iExists -[_]. rewrite tctx_hasty_val' // -(bi.exist_intro (S _)) bi.sep_assoc.
-    iFrame "Hdepth'". iCombine "ToObs Hproph" as "Hproph". iSplitR "Hproph".
-    - iFrame "HL'". iApply ("Hw" with "[-] [//]").
-      iNext. iExists (_::_::_). rewrite !heap_mapsto_vec_cons. iFrame.
-      iExists i, _, [_], _. rewrite -Hlen. auto.
-    - iApply (proph_obs_impl with "Hproph") => π /= [impl ?]. by apply impl.
+    iIntros ([Sztyb Wrt] Lk ??(?&?&[]))
+      "#LFT #TIME PROPH UNIQ #E $ [L L₊] /=(p & q &_) Obs".
+    iDestruct (closed_hasty with "p") as %?. iDestruct (closed_hasty with "q") as %?.
+    wp_apply (wp_hasty with "p"). iIntros (???) "⧖ ty".
+    iMod (Wrt with "LFT UNIQ E L ty") as (?->) "[(%vl & ↦ & tyb) Toty']".
+    iDestruct (ty_size_eq with "tyb") as "#>%Lenvl".
+    move: Lenvl. rewrite Sztyb. move: vl=> [|]; [done|]=>/= ? vl [= Lenvl].
+    rewrite heap_mapsto_vec_cons. iDestruct "↦" as "[>↦i ↦]". wp_write.
+    wp_bind p. iApply wp_wand; [by iApply wp_eval_path|]. iIntros (?->).
+    iMod (Lk with "LFT PROPH E L₊ tyb") as "Upd"; [done|]. wp_bind (_+ₗ_)%E.
+    iApply (wp_step_fupdN_persistent_time_receipt _ _ ∅ with "TIME ⧖ [Upd]");
+      [done..| |]. { iApply step_fupdN_with_emp. by rewrite difference_empty_L. }
+    wp_op. iIntros "[Obs' $] !>". iCombine "Obs Obs'" as "Obs".
+    wp_apply (wp_hasty with "q"). iIntros (???) "⧖' tyi".
+    iDestruct (ty_size_eq with "tyi") as %Sztyi.
+    move: (max_hlist_with_ge (λ _, ty_size) tyl i). rewrite -Sztyi -Lenvl /=.
+    case vl=>/=; [lia|]=> ?? _. rewrite heap_mapsto_vec_cons.
+    iDestruct "↦" as "[↦ ↦p]". iApply wp_fupd.
+    iApply (wp_persistent_time_receipt with "TIME ⧖'"); [done|]. wp_write.
+    iIntros "#⧖'". iMod ("Toty'" with "[↦i ↦ ↦p tyi] ⧖'") as "[$ ty']".
+    { iNext. iExists (_::_::_). rewrite !heap_mapsto_vec_cons.
+      iFrame "↦i ↦ ↦p". iExists _, _, [_], _. by iFrame. }
+    iModIntro. iExists -[_]. rewrite right_id.
+    iSplit. { iExists _, _. by iFrame "⧖' ty'". }
+    iApply proph_obs_impl; [|done]=>/= ?[? Imp]. by apply Imp.
   Qed.
 
-  Lemma type_sum_assign {E L 𝔅l ℭl 𝔄 𝔄' 𝔅 ℭ 𝔄l}
-        (ty' : type 𝔅) (tyl : typel 𝔄l) i (ty1 : type 𝔄) (ty1' : type 𝔄')
-        (C : cctx ℭ) (T : tctx 𝔅l) (T' : tctx ℭl) p1 p2 e gt st tr fr Φ:
-    Closed [] e → (0 ≤ i)%nat →
-    tctx_extract_ctx E L +[p1 ◁ ty1; p2 ◁ hnthb tyl i] T T' fr →
-    typed_write E L ty1 ty' ty1' (xsum_ty tyl) gt st →
-    leak' E L ty' Φ →
-    typed_body E L C ((p1 ◁ ty1') +:: T') e tr -∗
-    typed_body E L C T (p1 <-{Σ i} p2 ;; e)
-      (fr ∘ (λ post '(a -:: b -:: f), Φ (gt a) (tr post (st a (pinj i b) -:: f)))).
+  Lemma type_sum_assign {𝔄 𝔄' 𝔅 𝔅l ℭl 𝔇l 𝔈} (tyl: typel 𝔅l) (i: fin _)
+      (k: Z) (ty: type 𝔄) (tyb: type 𝔅) (ty': type 𝔄')
+      (T: tctx ℭl) (T': tctx 𝔇l) p q gt st Φ tr trx E L (C: cctx 𝔈) e :
+    Closed [] e → k = i → tctx_extract_ctx E L +[p ◁ ty; q ◁ tyl +!! i] T T' trx →
+    typed_write E L ty tyb ty' (Σ! tyl) gt st → leak' E L tyb Φ →
+    typed_body E L C (p ◁ ty' +:: T') e tr -∗
+    typed_body E L C T (p <-{Σ k} q;; e) (trx ∘ (λ post '(a -:: b' -:: dl),
+      Φ (gt a) (tr post (st a (pinj i b') -:: dl)))).
   Proof.
-    iIntros. iApply typed_body_tctx_incl; [done|]. via_tr_impl.
-    { iApply type_seq; by [eapply type_sum_assign_instr|solve_typing]. }
-    done.
+    iIntros (?->???) "e". iApply typed_body_tctx_incl; [done|].
+    iApply type_seq; [by eapply type_sum_assign_instr|apply tctx_incl_refl| |done].
+    by move=> ?[?[??]]/=.
   Qed.
 
-  Lemma type_sum_unit_instr {E L 𝔄 𝔄' 𝔅 𝔄l} (i: nat) (ty' : type 𝔅) (tyl: typel 𝔄l)
-                            (ty1: type 𝔄) (ty2: type 𝔄') p gt st eq:
-    hnthb tyl i = eq_rect _ _ unit_ty _ eq →
-    typed_write E L ty1 ty' ty2 (xsum_ty tyl) gt st →
-    typed_instr E L +[p ◁ ty1] (p <-{Σ i} ())
-    (λ _, +[p ◁ ty2]) (λ post '-[a], post -[st a (pinj i (eq_rect unitₛ _ () _ eq))]).
+  Lemma type_sum_unit_instr {𝔄 𝔄' 𝔅 𝔅l} (tyl: typel 𝔅l) (i: fin _)
+      (ty: type 𝔄) (tyb: type 𝔅) (ty': type 𝔄') f p gt st Φ E L :
+    typed_write E L ty tyb ty' (Σ! tyl) gt st → leak' E L tyb Φ →
+    subtype E L () (tyl +!! i) f →
+    typed_instr E L +[p ◁ ty] (p <-{Σ i} ()) (λ _, +[p ◁ ty'])
+      (λ post '-[a], Φ (gt a) (post -[st a (pinj i (f ()))])).
   Proof.
-    iIntros (Hty [Eq Hw] tid postπ [vπ []]) "#LFT #TIME #PROPH #UNIQ #HE $ HL [Hp _] Hproph".
-    wp_apply (wp_hasty with "Hp"). iIntros (depth v) "%Hv Hdepth Hty".
-    iMod (Hw with "LFT UNIQ HE HL Hty") as (l ->) "(H & Hw)". clear Hw.
-    iDestruct "H" as (vl) "(>H↦ & H)". iMod (ty'.(ty_size_eq) with "H") as "H".
-    destruct vl as [|? vl]; iDestruct "H" as %[= Hlen]; rewrite Eq //= in Hlen.
-    rewrite heap_mapsto_vec_cons -wp_fupd. iDestruct "H↦" as "[H↦0 H↦vl]".
-    iApply (wp_persistent_time_receipt with "TIME Hdepth")=>//.
-    wp_write. iIntros "#Hdepth". iExists -[_].
-    rewrite right_id bi.sep_assoc tctx_hasty_val' //. iSplitR "Hproph".
-    - rewrite -(bi.exist_intro (S _)). iFrame "Hdepth".
-      iApply ("Hw" with "[-] Hdepth"). iModIntro. iExists (_::_).
-      rewrite heap_mapsto_vec_cons. iFrame.
-      iExists i, (λ _, eq_rect _ _ () _ eq), [], _. rewrite Hty -Hlen.
-      iSplit; [done|]. clear Hty; destruct eq. iExists (const -[]). auto.
-    - by iApply (proph_obs_impl with "Hproph").
+    iIntros ([Sztyb Wrt] Lk Sub ??[?[]]) "#LFT #TIME PROPH UNIQ #E $ [L L₊] [p _] Obs".
+    iDestruct (Sub with "L") as "#In". iDestruct ("In" with "E") as "(%&_& #InOwn &_)".
+    wp_apply (wp_hasty with "p"). iIntros (???) "⧖ ty".
+    iMod (Wrt with "LFT UNIQ E L ty") as (?->) "[(%vl & ↦ & tyb) Toty']".
+    iDestruct (ty_size_eq with "tyb") as "#>%Lenvl".
+    move: Lenvl. rewrite Sztyb. move: vl=> [|]; [done|]=>/= ? vl [= Lenvl].
+    rewrite heap_mapsto_vec_cons. iDestruct "↦" as "[>↦i ↦]". wp_bind (_<-_)%E.
+    iApply (wp_persistent_time_receipt with "TIME ⧖"); [done|]. wp_write.
+    iIntros "#⧖". iMod (Lk with "LFT PROPH E L₊ tyb") as "Upd"; [done|].
+    iApply (wp_step_fupdN_persistent_time_receipt _ _ ∅ with "TIME ⧖ [Upd]");
+      [done..| |].
+    { iApply step_fupdN_with_emp. rewrite difference_empty_L /=.
+      by iIntros "!>!>!>!>!>!>!>". }
+    do 2 wp_seq. iIntros "[Obs' $]". iCombine "Obs Obs'" as "Obs".
+    iDestruct ("InOwn" $! (const ()) _ _ [] with "[]") as "tyi".
+    { by iExists (const -[]). }
+    iMod ("Toty'" with "[↦i ↦ tyi] ⧖") as "[$ ty']".
+    { iNext. iExists (_::_). rewrite !heap_mapsto_vec_cons. iFrame "↦i ↦".
+      iExists i, _, [], _. iFrame "tyi". by rewrite/= Lenvl. }
+    iModIntro. iExists -[_]. rewrite right_id.
+    iSplit. { iExists _, _. by iFrame "⧖ ty'". }
+    iApply proph_obs_impl; [|done]=>/= ?[? Imp]. by apply Imp.
   Qed.
 
-  Lemma type_sum_unit {E L 𝔄 𝔄' 𝔅 ℭ 𝔄l 𝔅l ℭl} (ty' : type 𝔅) (tyl : typel 𝔄l) i (ty1 : type 𝔄)
-                      (ty1' : type 𝔄') (C : cctx ℭ) (T : tctx 𝔅l) (T' : tctx ℭl) p e
-                      gt st fr tr (eq : ()%ST = lnthe 𝔄l i) :
-    Closed [] e → (0 ≤ i)%nat →
-    tctx_extract_ctx E L +[p ◁ ty1] T T' fr →
-    hnthb tyl i = eq_rect _ _ unit_ty _ eq →
-    typed_write E L ty1 ty' ty1' (xsum_ty tyl) gt st →
-    typed_body E L C (p ◁ ty1' +:: T') e tr -∗
-    typed_body E L C T (p <-{Σ i} () ;; e)
-      (fr ∘ (λ post '(a -:: f), tr post (st a (pinj i (eq_rect unitₛ _ () _ eq)) -:: f))).
+  Lemma type_sum_unit {𝔄 𝔄' 𝔅 𝔅l ℭl 𝔇l 𝔈} (tyl: typel 𝔅l) (i: fin _) (k: Z)
+      (ty: type 𝔄) (tyb: type 𝔅) (ty': type 𝔄') (T: tctx ℭl) (T': tctx 𝔇l)
+      f trx tr p gt st e Φ E L (C: cctx 𝔈) :
+    Closed [] e → k = i → tctx_extract_ctx E L +[p ◁ ty] T T' trx →
+    typed_write E L ty tyb ty' (Σ! tyl) gt st → leak' E L tyb Φ →
+    subtype E L () (tyl +!! i) f →
+    typed_body E L C (p ◁ ty' +:: T') e tr -∗
+    typed_body E L C T (p <-{Σ k} ();; e) (trx ∘
+      (λ post '(a -:: dl), Φ (gt a) (tr post (st a (pinj i (f ())) -:: dl)))).
   Proof.
-    iIntros (???) "* **". iApply typed_body_tctx_incl; [done|].
-    iApply type_seq; [by eapply type_sum_unit_instr|solve_extract| |done]. done.
+    iIntros (?->????) "e". iApply typed_body_tctx_incl; [done|].
+    iApply type_seq; [by eapply type_sum_unit_instr|by apply tctx_incl_refl| |done].
+    by move=> ?[??]/=.
   Qed.
 
-  Lemma type_sum_memcpy_instr {E L 𝔄l 𝔄 𝔄' 𝔅 𝔅' ℭ} (i : nat) (ty' : type ℭ) (tyl : typel 𝔄l)
-    (ty1 : type 𝔄) (ty1' : type 𝔄') (ty2 : type 𝔅) (ty2' : type 𝔅') p1 p2 gt st rd wt Φ:
-    let ty := hnthb tyl i in leak' E L ty' Φ →
-    typed_write E L ty1 ty' ty1' (xsum_ty tyl) gt st →
-    typed_read E L ty2 ty ty2' rd wt →
-    typed_instr E L +[p1 ◁ ty1; p2 ◁ ty2]
-      (p1 <-{ty.(ty_size),Σ i} !p2) (λ _, +[p1 ◁ ty1'; p2 ◁ ty2'])
-      (λ post '-[a; b], Φ (gt a) (post -[st a (pinj i (rd b)); wt b])).
+  Lemma type_sum_memcpy_instr {𝔄 𝔄' 𝔅 𝔅' ℭ ℭl} (tyl: typel ℭl) (i: fin _)
+      (tyw: type 𝔄) (tyw': type 𝔄') (tyr: type 𝔅) (tyr': type 𝔅')
+      (tyb: type ℭ) p q gtw stw gtr str Φ E L :
+    typed_write E L tyw tyb tyw' (Σ! tyl) gtw stw → leak' E L tyb Φ →
+    typed_read E L tyr (tyl +!! i) tyr' gtr str →
+    typed_instr E L +[p ◁ tyw; q ◁ tyr]
+      (p <-{(tyl +!! i).(ty_size),Σ i} !q) (λ _, +[p ◁ tyw'; q ◁ tyr'])
+      (λ post '-[a; b], Φ (gtw a) (post -[stw a (pinj i (gtr b)); str b])).
   Proof.
-    iIntros (ty Lk [Eq Hw] Hr tid postπ (vπ & wπ & []))
-      "#LFT #TIME #PROPH #UNIQ #HE Htl (HL1 & HL2 & HL3) (Hp1 & Hp2 & _) Hproph".
-    iDestruct (closed_hasty with "Hp1") as "%". iDestruct (closed_hasty with "Hp2") as "%".
-    wp_apply (wp_hasty with "Hp1"). iIntros (v1 depth1) "%Hv1 Hdepth1 Hty1".
-    iDestruct "Hp2" as (v2 depth2) "(%Hv2 & Hdepth2 & Hty2)".
-    iCombine "Hdepth1 Hdepth2" as "#Hdepth".
-    rewrite !(ty_own_depth_mono _ _ (depth1 `max` depth2)); [|lia..].
-    iMod (Hw with "LFT UNIQ HE HL1 Hty1") as (l1 ->) "(H & Hw)".
-    iDestruct "H" as (?) "(>H↦ & Leaked)".
-    iAssert (▷ (ty_own ty' (gt ∘ vπ) (depth1 `max` depth2) tid vl ∗
-      ⌜length vl = ty_size ty'⌝))%I with "[Leaked]" as "[Leaked >%Hlen]".
-    { iNext. iDestruct (ty_size_eq with "Leaked") as %<-. by iFrame. }
-    destruct vl as [|? vl]; rewrite -Hlen //= in Eq.
-    rewrite heap_mapsto_vec_cons -wp_fupd. iDestruct "H↦" as "[H↦0 H↦vl1]". wp_write.
-    wp_bind p1. iApply (wp_wand with "[]"); first by iApply (wp_eval_path).
-    iIntros (? ->). wp_op. wp_bind p2.
-    iApply (wp_wand with "[]"); first by iApply (wp_eval_path). iIntros (? ->).
-    iMod (Hr with "LFT HE Htl HL2 Hty2") as (l2 vl2 q) "(% & H↦2 & Hty & Hr)" => //=.
-    iDestruct (Lk (⊤ ∖ (⊤ ∖ ↑lftN ∖ ↑prophN)) with "LFT PROPH HE HL3 Leaked")
-      as "ToObs"; first set_solver.
-    iApply (wp_step_fupdN_persistent_time_receipt _ _ (⊤ ∖ ↑lftN ∖ ↑prophN)
-      with "TIME Hdepth [ToObs]")=>//.
-    { by iApply step_fupdN_with_emp. }
-    clear Hr. subst. assert (ty.(ty_size) ≤ length vl).
-    { move: Eq => [= ->]. clear. generalize dependent i.
-      elim tyl => //= > + [|i] => [_|/(_ i)]; lia. }
-    rewrite -(take_drop ty.(ty_size) vl) heap_mapsto_vec_app.
-    iDestruct "H↦vl1" as "[H↦vl1 H↦pad]".
-    iDestruct (ty_size_eq with "Hty") as "#>%Hvl2Len".
-    iApply (wp_persistent_time_receipt with "TIME Hdepth"); first solve_ndisj.
-    iApply (wp_memcpy with "[$H↦vl1 $H↦2]"); [|lia|].
-    { rewrite take_length. lia. }
-    iNext; iIntros "[H↦vl1 H↦2] #Hdepth' [ToObs HL'] !>". iExists -[_; _].
-    rewrite right_id !tctx_hasty_val' //.
-    iMod ("Hr" with "H↦2") as "($ & HL & Hty2)". iCombine "HL HL'" as "$".
-    iCombine "ToObs Hproph" as "Hproph".
-    iMod ("Hw" with "[-Hty2 Hproph] Hdepth'") as "[$ Hty]"; last first. iSplitR "Hproph".
-    { iSplitL "Hty"; [eauto with iFrame|]. iExists _. iFrame.
-      iApply persistent_time_receipt_mono; [|done]. lia. }
-    { iApply (proph_obs_impl with "Hproph") => /= π [impl post]. apply impl. apply post. }
-    iNext. rewrite split_sum_mt /is_pad. iExists i, _. iFrame.
-    iSplitR; [done|iSplitL "H↦pad"].
-    - rewrite (shift_loc_assoc_nat _ 1) take_length Nat.min_l; last lia.
-      iExists _. iFrame. rewrite /= drop_length. iPureIntro. rewrite -Hvl2Len. lia.
-    - iExists _. iFrame.
+    set tyi := tyl +!! i. iIntros ([Sztyb Wrt] Lk Rd ??(?&?&[]))
+      "#LFT #TIME PROPH UNIQ #E Na [L L₊] /=(p & q &_) Obs".
+    iDestruct (closed_hasty with "p") as %?. iDestruct (closed_hasty with "q") as %?.
+    wp_apply (wp_hasty with "p"). iIntros (???) "#⧖ tyw".
+    iMod (Wrt with "LFT UNIQ E L tyw") as (?->) "[(%vl & ↦ & tyb) Totyw']".
+    iDestruct (ty_size_eq with "tyb") as "#>%Lenvl".
+    move: Lenvl. rewrite Sztyb. move: vl=> [|]; [done|]=>/= ? vl [= Lenvl].
+    rewrite heap_mapsto_vec_cons. iDestruct "↦" as "[>↦i ↦]". wp_write.
+    wp_bind p. iApply wp_wand; [by iApply wp_eval_path|]. iIntros (?->).
+    iMod (Lk with "LFT PROPH E L₊ tyb") as "Upd"; [done|]. wp_bind (_+ₗ_)%E.
+    iApply (wp_step_fupdN_persistent_time_receipt _ _ ∅ with "TIME ⧖ [Upd]");
+      [done..| |]. { iApply step_fupdN_with_emp. by rewrite difference_empty_L. }
+    wp_op. iIntros "[Obs' L₊] !>". iCombine "Obs Obs'" as "Obs".
+    wp_apply (wp_hasty with "q"). iIntros (???) "#⧖' tyr".
+    iMod (Rd with "LFT E Na L₊ tyr") as (? vl' ?->) "(↦' & tyi & Totyr')".
+    iDestruct (ty_size_eq with "tyi") as "#>%Lenvl'".
+    move: (max_hlist_with_ge (λ _, ty_size) tyl i).
+    set tyisz := tyi.(ty_size). set maxsz := max_hlist_with _ _=> ?.
+    have LenvlAdd: length vl = tyisz + (maxsz - tyisz) by lia.
+    move: LenvlAdd=> /app_length_ex[wl[wl'[->[Lenwl ?]]]].
+    rewrite heap_mapsto_vec_app Lenwl. iDestruct "↦" as "[↦ ↦p]". iApply wp_fupd.
+    iApply (wp_persistent_time_receipt with "TIME ⧖'"); [done|].
+    iApply (wp_memcpy with "[$↦ $↦']"); [lia..|]. iIntros "!> [↦ ↦'] #⧖'S".
+    iMod ("Totyr'" with "↦'") as "($&$& tyr')".
+    iMod ("Totyw'" with "[↦i ↦ ↦p tyi] ⧖'S") as "($& tyw')".
+    { iNext. iExists (_::_++_). rewrite heap_mapsto_vec_cons heap_mapsto_vec_app.
+      rewrite /tyisz -Lenvl'. iFrame "↦i ↦ ↦p". iExists _, _, _, _. iFrame "tyi".
+      iPureIntro. do 2 (split; [done|]). rewrite/= app_length. lia. }
+    iModIntro. iExists -[λ π, _;λ π, _]. rewrite right_id. iSplit; last first.
+    { iApply proph_obs_impl; [|done]=>/= ?[? Imp]. by apply Imp. }
+    iSplitL "tyw'"; iExists _, _; (iSplit; [done|]); by iFrame.
   Qed.
 
-  Lemma type_sum_memcpy {E L 𝔄l 𝔄 𝔄' 𝔅 𝔅' ℭ 𝔇 𝔅l ℭl} (ty' : type ℭ) (tyl : typel 𝔄l) i
-                        (ty1 : type 𝔄) (ty2 : type 𝔅) n (ty1' : type 𝔄')
-                        (ty2' : type 𝔅') (C : cctx 𝔇) (T : tctx 𝔅l) (T' : tctx ℭl) p1 p2
-                        e fr tr gt st rd wt Φ:
-    let ty := hnthb tyl i in
-    leak' E L ty' Φ → Closed [] e → (0 ≤ i)%nat →
-    tctx_extract_ctx E L +[p1 ◁ ty1; p2 ◁ ty2] T T' fr →
-    typed_write E L ty1 ty' ty1' (xsum_ty tyl) gt st →
-    typed_read E L ty2 ty ty2' rd wt →
-    Z.of_nat ty.(ty_size) = n →
-    typed_body E L C ((p1 ◁ ty1') +:: (p2 ◁ ty2') +:: T') e tr -∗
-    typed_body E L C T (p1 <-{n,Σ i} !p2 ;; e)
-      (fr ∘ (λ post '(a -:: b -:: f),
-        Φ (gt a) (tr post (st a (pinj i (rd b)) -:: wt b -:: f)))).
+  Lemma type_sum_memcpy {𝔄 𝔄' 𝔅 𝔅' ℭ ℭl 𝔇l 𝔈l 𝔉} (tyl: typel ℭl) (i: fin _) (k: Z)
+      (tyw: type 𝔄) (tyw': type 𝔄') (tyr: type 𝔅) (tyr': type 𝔅') (tyb: type ℭ)
+      (T: tctx 𝔇l) (T': tctx 𝔈l) p q gtw stw gtr str trx tr e Φ E L (C: cctx 𝔉) :
+    Closed [] e → k = i → tctx_extract_ctx E L +[p ◁ tyw; q ◁ tyr] T T' trx →
+    typed_write E L tyw tyb tyw' (Σ! tyl) gtw stw → leak' E L tyb Φ →
+    typed_read E L tyr (tyl +!! i) tyr' gtr str →
+    typed_body E L C (p ◁ tyw' +:: q ◁ tyr' +:: T') e tr -∗
+    typed_body E L C T (p <-{(tyl +!! i).(ty_size),Σ i} !q;; e)
+      (trx ∘ (λ post '(a -:: b -:: el),
+        Φ (gtw a) (tr post (stw a (pinj i (gtr b)) -:: str b -:: el)))).
   Proof.
-    iIntros (??????? <-) "* **". iApply typed_body_tctx_incl; [done|].
-    iApply type_seq; [by eapply type_sum_memcpy_instr|solve_extract| |done]. done.
+    iIntros (?->????) "e". iApply typed_body_tctx_incl; [done|].
+    iApply type_seq; [by eapply type_sum_memcpy_instr|by apply tctx_incl_refl| |done].
+    by move=> ?[?[??]]/=.
   Qed.
 
-  Lemma ty_outlives_E_elctx_sat_sum {𝔄l} E L (tyl : typel 𝔄l) α:
-    elctx_sat E L (tyl_outlives_E tyl α) →
-    elctx_sat E L (ty_outlives_E (xsum_ty tyl) α).
+  Lemma ty_outlives_E_elctx_sat_sum {𝔄l} E L (tyl: typel 𝔄l) κ :
+    elctx_sat E L (tyl_outlives_E tyl κ) →
+    elctx_sat E L (ty_outlives_E (Σ! tyl) κ).
   Proof.
-    intro Hsat. eapply eq_ind; [done|]. clear Hsat.
+    move=> Sat. eapply eq_ind; [done|]. clear Sat.
     rewrite /tyl_outlives_E /ty_outlives_E /=.
     induction tyl as [|???? IH]=>//=. by rewrite IH fmap_app.
   Qed.
-End case.
+End type_sum.
 
 Global Hint Resolve ty_outlives_E_elctx_sat_sum : lrust_typing.
